src/PlutusIR/Semantics/Static/normaliser/STLC_norm_completeness.v
@@ -1,0 +1,65 @@
+From PlutusCert Require Import STLC_named STLC_normalisation SN_STLC_named STLC_named_typing.
+Require Import Coq.Lists.List.
+Import ListNotations.
+
+(* sound: if function, then relation*)
+(* complete: if relation, then function*)
+
+(* Lemma strong_normalization_SN :
+  forall E s T (H : SN_STLC_named.has_type E s T), strong_normalization H = SN s.
+Proof.
+  (* This requires proving equivalence, likely with the definition of `strong_normalization`. *)
+Admitted. *)
+
+Theorem norm_complete Δ K (t tn : term) (Hwt : SN_STLC_named.has_type Δ t K) :
+    normalise t tn -> normalizer Hwt = tn.
+Proof.
+    intros HnormR.
+    generalize dependent Δ.
+    generalize dependent K.
+    induction HnormR; intros K' Δ Hwt; subst; auto.
+    - inversion Hwt; subst.
+
+      (* IHHnormR2:
+        K0 is the type of T2, which is K1
+      *)
+      specialize (IHHnormR2 K1 Δ H4).
+
+      (* IHHnormR1 K0 is the type of T1, which is K1 -> K'*)
+      specialize (IHHnormR1 (tp_arrow K1 K') Δ H2).
+
+            (* IHHnormR3:
+        K0 is the type of substituteTCA bX T2n T1n, hence it is the type of T1n
+        which should have the same type as T1.
+        Which is K1 -> K'.
+        *)
+      specialize (IHHnormR3 (tp_arrow K1 K') Δ).
+
+      admit.
+    - admit.
+    - 
+      (* specialize (IHHnormR ((bX, K)::Δ)). *)
+      inversion Hwt; subst.
+      specialize (IHHnormR K2 ((bX, K)::Δ) H4).
+      admit.
+    - unfold normalizer.
+      inversion Hwt; subst.
+      (* unfold normalizer''. *)
+      simpl.
+      remember Hwt as Hwt'; clear HeqHwt'.
+      assert (SN (tmvar X)).
+      {
+        apply strong_normalization in Hwt'.
+        
+        apply Hwt'.
+      }
+      admit.
+      
+      
+      
+Admitted.
+
+Theorem norm_sound Δ T (t tn : term) (Hwt : SN_STLC_named.has_type Δ t T) :
+    normalizer Hwt = tn -> normalise t tn.
+Proof.
+Admitted.
