src/PlutusIR/Semantics/Static/normaliser/STLC_normalisation.v
@@ -1,4 +1,6 @@
-From PlutusCert Require Import STLC_named.
+Require Import Strings.String.
+
+From PlutusCert Require Import STLC_named STLC_named_typing.
 
 (** Normal types *)
 Inductive normal_Ty : term -> Prop :=
@@ -26,20 +28,6 @@ Combined Scheme normal_Ty__multind from
 
 #[export] Hint Constructors normal_Ty neutral_Ty : core.
 
-Fixpoint is_normal (t : term) : bool :=
-  match t with
-  | tmlam X K T => is_normal T
-  | tmvar X => true
-  | tmapp T1 T2 => is_neutral T1 && is_normal T2
-  end
-
-with is_neutral (t : term) : bool :=
-  match t with
-  | tmvar X => true
-  | tmapp T1 T2 => is_neutral T1 && is_normal T2
-  | _ => false
-  end.
-
 (** Type normalisation *)
 Inductive normalise : term -> term -> Prop :=
   | N_BetaReduce : forall bX K T1 T2 T1n T2n T,
@@ -60,5 +48,3 @@ Inductive normalise : term -> term -> Prop :=
   .
 
 #[export] Hint Constructors normalise : core.
-
-
